src/Examples/Mixed/Analyse_Dispatch.thy
@@ -417,6 +417,7 @@ code_identifier
 | code_module DG_Framework \<rightharpoonup> (OCaml) Core
 | code_module Abstract_Checks \<rightharpoonup> (OCaml) Core
 | code_module Exec_DG_Bridge \<rightharpoonup> (OCaml) Core
+| code_module DG_Base_Exec \<rightharpoonup> (OCaml) Core
 | code_module Sign_Arithmetic \<rightharpoonup> (OCaml) Core
 | code_module Sign_Special \<rightharpoonup> (OCaml) Core
 | code_module Sign_Backward \<rightharpoonup> (OCaml) Core
