src/VIMP/VIMP_Settings.thy
@@ -1,0 +1,7 @@
+theory VIMP_Settings
+  imports Main
+begin
+
+declare [[show_sorts, show_consts, goals_limit = 50]]
+
+end
